A12Kernel.lean
@@ -102,6 +102,7 @@ import A12Kernel.Elaboration.StringComputationTable
 import A12Kernel.Elaboration.StringComputationRun
 import A12Kernel.Elaboration.StringComputationRunRelation
 import A12Kernel.Elaboration.StringComputationRunResult
+import A12Kernel.Elaboration.StringComputationRunApplication
 import A12Kernel.Elaboration.EnumerationComputation
 import A12Kernel.Elaboration.EnumerationFirstFilledComputation
 import A12Kernel.Elaboration.NumericValidation
